I made various cosmetic changes to the theories including better automation for proofs about variables (utp_var). More notably, the equivalence between the simplified and algebraic definition of sequential composition is proved and the conditional operator was added too. A new theory utp_laws was added to comprise algebraic laws. Sorrys have been discharged for pending proofs about SS1 and SS2 in utp_rel.

theories/generic/utp_rel.thy
@@ -16,13 +16,36 @@ begin
 subsection {* Restrictions *}
 
 definition NON_REL_VAR :: "'TYPE VAR set" where
-"NON_REL_VAR = VAR - (DASHED \<union> UNDASHED)"
+"NON_REL_VAR = VAR - (UNDASHED \<union> DASHED)"
 
 definition COMPOSABLE ::
   "(('VALUE, 'TYPE) BINDING \<times>
     ('VALUE, 'TYPE) BINDING) set" where
 "COMPOSABLE = {(b1, b2) .
    (\<forall> v \<in> UNDASHED . b1(dash v) = b2 v) \<and> b1 \<cong> b2 on NON_REL_VAR}"
+
+definition UNREST ::
+  "('TYPE VAR) set \<Rightarrow> ('VALUE, 'TYPE) PREDICATE \<Rightarrow> bool" where
+"UNREST vs p \<longleftrightarrow> (\<forall> b1 \<in> p . \<forall> b2 \<in> WF_BINDING . b1 \<oplus> b2 on vs \<in> p)"
+
+subsection {* Substitutions *}
+
+text {* The substitution @{term "SS"} swaps dashed and undashed variables. *}
+
+definition SS :: "'TYPE VAR \<Rightarrow> 'TYPE VAR" where
+"SS = (\<lambda> v .
+   if v \<in> UNDASHED then (dash v) else
+   if v \<in> DASHED then (undash v) else v)"
+
+definition SS1 :: "'TYPE VAR \<Rightarrow> 'TYPE VAR" where
+"SS1 = (\<lambda> v .
+ if (v \<in> DASHED) then (dash v) else
+ if (v \<in> DASHED_TWICE) then (undash v) else v)"
+
+definition SS2 :: "'TYPE VAR \<Rightarrow> 'TYPE VAR" where
+"SS2 = (\<lambda> v .
+ if v \<in> UNDASHED then dash (dash v) else
+ if v \<in> DASHED_TWICE then undash (undash v) else v)"
 
 subsection {* Operators *}
 
@@ -33,7 +56,7 @@ definition SkipR :: "('VALUE, 'TYPE) PREDICATE" where
 
 notation SkipR ("II")
 
-subsubsection {* Sequential Composition *}
+subsubsection {* Sequence *}
 
 definition SemiR ::
   "('VALUE, 'TYPE) PREDICATE \<Rightarrow>
@@ -48,7 +71,296 @@ definition SemiR ::
 
 notation SemiR (infixr ";" 140)
 
+text {* Algebraic version of sequential composition *}
+
+definition SemiR2 ::
+  "('VALUE, 'TYPE) PREDICATE \<Rightarrow>
+   ('VALUE, 'TYPE) PREDICATE \<Rightarrow>
+   ('VALUE, 'TYPE) PREDICATE" where
+"p1 \<in> WF_PREDICATE \<and>
+ p2 \<in> WF_PREDICATE \<and>
+ UNREST DASHED_TWICE p1 \<and>
+ UNREST DASHED_TWICE p2 \<longrightarrow>
+ SemiR2 p1 p2 = (\<exists>p DASHED_TWICE . p1[SS1] \<and>p p2[SS2])"
+
+subsubsection {* Conditional *}
+
+text {* Should we impose a constraint on b for it to be a condition? *}
+
+definition CondR ::
+  "('VALUE, 'TYPE) PREDICATE \<Rightarrow>
+   ('VALUE, 'TYPE) PREDICATE \<Rightarrow>
+   ('VALUE, 'TYPE) PREDICATE \<Rightarrow>
+   ('VALUE, 'TYPE) PREDICATE" where
+"p1 \<in> WF_PREDICATE \<and>
+ p2 \<in> WF_PREDICATE \<and>
+ b \<in> WF_PREDICATE \<longrightarrow>
+ CondR p1 b p2 = (b \<and>p p1) \<or>p (\<not>p b \<and>p p2)"
+
+notation CondR ("_ \<triangleleft> _ \<triangleright> _")
+
 subsection {* Theorems *}
+
+subsubsection {* Substitution Theorems *}
+
+text {* Theorems for @{term SS} *}
+
+theorem SS_UNDASHED_app :
+"\<lbrakk>x \<in> UNDASHED\<rbrakk> \<Longrightarrow> SS x = dash x"
+apply (simp add: SS_def)
+done
+
+theorem SS_DASHED_app :
+"\<lbrakk>x \<in> DASHED\<rbrakk> \<Longrightarrow> SS x = undash x"
+apply (simp add: SS_def)
+apply (simp add: var_defs)
+done
+
+theorem SS_DASHED_TWICE_app :
+"\<lbrakk>x \<in> DASHED_TWICE\<rbrakk> \<Longrightarrow> SS x = x"
+apply (simp add: SS_def)
+apply (simp add: var_defs)
+done
+
+theorem SS_ident_app :
+"\<lbrakk>\<not> x \<in> UNDASHED; \<not> x \<in> DASHED\<rbrakk> \<Longrightarrow> SS x = x"
+apply (simp add: SS_def)
+done
+
+theorems SS_simps =
+  SS_UNDASHED_app
+  SS_DASHED_app
+  SS_DASHED_TWICE_app
+  SS_ident_app
+
+theorem SS_VAR_SUBST [closure] :
+"SS \<in> VAR_SUBST"
+apply (simp add: VAR_SUBST_def)
+apply (simp add: bij_def)
+apply (safe)
+apply (simp_all)
+-- {* Subgoal 1 *}
+apply (simp add: inj_on_def)
+apply (simp add: SS_def)
+apply (safe)
+apply (auto)
+-- {* Subgoal 1.1 *}
+apply (insert undash_inj_on_DASHED) [1]
+apply (simp add: inj_on_eq_iff)
+-- {* Subgoal 1.2 *}
+apply (insert dash_inj) [1]
+apply (simp add: inj_on_eq_iff)
+-- {* Subgoal 2 *}
+apply (simp add: image_def)
+apply (rule_tac x = "SS x" in exI)
+apply (simp add: SS_def)
+apply (auto) [1]
+  -- {* Subgoal 4 *}
+apply (simp add: SS_def)
+done
+
+theorem SS_VAR_SUBST_ON [closure] :
+"SS \<in> VAR_SUBST_ON (UNDASHED \<union> DASHED)"
+apply (simp add: VAR_SUBST_ON_def)
+apply (simp add: SS_VAR_SUBST)
+apply (simp add: SS_def)
+done
+
+theorem SS_VAR_SUBST_INV [closure] :
+"SS \<in> VAR_SUBST_INV"
+apply (simp add: VAR_SUBST_INV_def)
+apply (simp add: SS_VAR_SUBST)
+apply (rule sym [OF inv_equality])
+apply (simp_all add: SS_def)
+apply (auto)
+done
+
+theorem SS_inv [simp] :
+"inv SS = SS"
+apply (insert SS_VAR_SUBST_INV)
+apply (simp add: VAR_SUBST_INV_def)
+done
+
+theorem SS_DASHED_member :
+"x \<in> DASHED \<Longrightarrow> \<not> SS x \<in> DASHED"
+apply (simp add: SS_def)
+apply (simp add: var_defs)
+done
+
+text {* Theorems for @{term SS1} *}
+
+theorem SS1_UNDASHED_app :
+"\<lbrakk>x \<in> UNDASHED\<rbrakk> \<Longrightarrow> SS1 x = x"
+apply (simp add: SS1_def)
+done
+
+theorem SS1_DASHED_app :
+"\<lbrakk>x \<in> DASHED\<rbrakk> \<Longrightarrow> SS1 x = dash x"
+apply (simp add: SS1_def)
+done
+
+theorem SS1_DASHED_TWICE_app :
+"\<lbrakk>x \<in> DASHED_TWICE\<rbrakk> \<Longrightarrow> SS1 x = undash x"
+apply (simp add: SS1_def)
+apply (simp add: var_defs)
+done
+
+theorem SS1_ident_app :
+"\<lbrakk>\<not> x \<in> DASHED; \<not> x \<in> DASHED_TWICE\<rbrakk> \<Longrightarrow> SS1 x = x"
+apply (simp add: SS1_def)
+done
+
+theorems SS1_simps =
+  SS1_UNDASHED_app
+  SS1_DASHED_app
+  SS1_DASHED_TWICE_app
+  SS1_ident_app
+
+theorem SS1_VAR_SUBST [closure] :
+"SS1 \<in> VAR_SUBST"
+apply (simp add: VAR_SUBST_def)
+apply (simp add: bij_def)
+apply (safe)
+apply (simp_all)
+-- {* Subgoal 1 *}
+apply (simp add: inj_on_def)
+apply (simp add: SS1_def)
+apply (safe)
+apply (auto)
+-- {* Subgoal 1.1 *}
+apply (insert undash_inj_on_DASHED_TWICE) [1]
+apply (simp add: inj_on_eq_iff)
+-- {* Subgoal 1.2 *}
+apply (insert dash_inj) [1]
+apply (simp add: inj_on_eq_iff)
+-- {* Subgoal 2 *}
+apply (simp add: image_def)
+apply (rule_tac x = "SS1 x" in exI)
+apply (simp add: SS1_def)
+apply (auto) [1]
+  -- {* Subgoal 4 *}
+apply (simp add: SS1_def)
+done
+
+theorem SS1_VAR_SUBST_ON [closure] :
+"SS1 \<in> VAR_SUBST_ON (DASHED \<union> DASHED_TWICE)"
+apply (simp add: VAR_SUBST_ON_def)
+apply (simp add: SS1_VAR_SUBST)
+apply (simp add: SS1_def)
+done
+
+theorem SS1_VAR_SUBST_INV [closure] :
+"SS1 \<in> VAR_SUBST_INV"
+apply (simp add: VAR_SUBST_INV_def)
+apply (simp add: SS1_VAR_SUBST)
+apply (rule sym [OF inv_equality])
+apply (simp_all add: SS1_def)
+apply (auto)
+done
+
+theorem SS1_inv [simp] :
+"inv SS1 = SS1"
+apply (insert SS1_VAR_SUBST_INV)
+apply (simp add: VAR_SUBST_INV_def)
+done
+
+text {* Theorems for @{term SS2} *}
+
+theorem SS2_DASHED_app :
+"x \<in> DASHED \<Longrightarrow> SS2 x = x"
+apply (simp add: SS2_def)
+apply (simp add: var_defs)
+done
+
+theorem SS2_UNDASHED_app :
+"x \<in> UNDASHED \<Longrightarrow> SS2 x = dash (dash x)"
+apply (simp add: SS2_def)
+done
+
+theorem SS2_DASHED_TWICE_app :
+"\<lbrakk>x \<in> DASHED_TWICE\<rbrakk> \<Longrightarrow> SS2 x =  undash (undash x)"
+apply (simp add: SS2_def)
+apply (simp add: var_defs)
+done
+
+theorem SS2_ident_app :
+"\<lbrakk>\<not> x \<in> UNDASHED; \<not> x \<in> DASHED_TWICE\<rbrakk> \<Longrightarrow> SS2 x = x"
+apply (simp add: SS2_def)
+done
+
+theorems SS2_simps =
+  SS2_UNDASHED_app
+  SS2_DASHED_app
+  SS2_DASHED_TWICE_app
+  SS2_ident_app
+
+theorem SS2_VAR_SUBST [closure] :
+"SS2 \<in> VAR_SUBST"
+apply (simp add: VAR_SUBST_def)
+apply (simp add: bij_def)
+apply (safe)
+apply (simp_all)
+-- {* Subgoal 1 *}
+apply (simp add: inj_on_def)
+apply (simp add: SS2_def)
+apply (safe)
+apply (auto)
+-- {* Subgoal 1.1 *}
+apply (insert undash_inj_on_DASHED undash_inj_on_DASHED_TWICE) [1]
+apply (simp add: inj_on_eq_iff)
+-- {* Subgoal 1.2 *}
+apply (insert dash_inj) [1]
+apply (simp add: inj_on_eq_iff)
+-- {* Subgoal 2 *}
+apply (simp add: image_def)
+apply (rule_tac x = "SS2 x" in exI)
+apply (simp add: SS2_def)
+apply (auto) [1]
+  -- {* Subgoal 4 *}
+apply (simp add: SS2_def)
+done
+
+theorem SS2_VAR_SUBST_ON [closure] :
+"SS2 \<in> VAR_SUBST_ON (UNDASHED \<union> DASHED_TWICE)"
+apply (simp add: VAR_SUBST_ON_def)
+apply (simp add: SS2_VAR_SUBST)
+apply (simp add: SS2_def)
+done
+
+theorem SS2_VAR_SUBST_INV [closure] :
+"SS2 \<in> VAR_SUBST_INV"
+apply (simp add: VAR_SUBST_INV_def)
+apply (simp add: SS2_VAR_SUBST)
+apply (rule sym [OF inv_equality])
+apply (simp_all add: SS2_def)
+apply (auto)
+done
+
+theorem SS2_inv [simp] :
+"inv SS2 = SS2"
+apply (insert SS2_VAR_SUBST_INV)
+apply (simp add: VAR_SUBST_INV_def)
+done
+
+subsubsection {* Restriction Theorems *}
+
+theorem UNREST_member [intro] :
+"\<lbrakk>p \<in> WF_PREDICATE; b \<in> p; UNREST vs p; b' \<in> WF_BINDING\<rbrakk> \<Longrightarrow>
+ (b \<oplus> b' on vs) \<in> p"
+apply (simp add: UNREST_def)
+done
+
+theorem COMPOSABLE_dash [intro] :
+"\<lbrakk>(b1, b2) \<in> COMPOSABLE; x \<in> UNDASHED\<rbrakk> \<Longrightarrow> b1(dash x) = b2 x"
+apply (simp add: COMPOSABLE_def)
+done
+
+theorem COMPOSABLE_ident [intro] :
+"\<lbrakk>(b1, b2) \<in> COMPOSABLE; \<not> x \<in> UNDASHED; \<not> x \<in> DASHED\<rbrakk> \<Longrightarrow> b1 x = b2 x"
+apply (simp only: COMPOSABLE_def)
+apply (simp add: NON_REL_VAR_def)
+apply (simp add: binding_equiv_def)
+done
 
 subsubsection {* Closure Theorems *}
 
@@ -57,6 +369,15 @@ theorem SkipR_closure [closure] :
 apply (simp add: SkipR_def)
 apply (simp add: WF_PREDICATE_def)
 apply (auto)
+done
+
+theorem CondR_closure [closure] :
+"p1 \<in> WF_PREDICATE \<and>
+ p2 \<in> WF_PREDICATE \<and>
+ b \<in> WF_PREDICATE \<longrightarrow>
+ p1 \<triangleleft> b \<triangleright> p2 \<in> WF_PREDICATE"
+apply (simp add: CondR_def)
+apply (simp add: closure)
 done
 
 theorem SemiR_closure [closure] :
@@ -68,18 +389,99 @@ apply (simp add: WF_PREDICATE_def)
 apply (auto)
 done
 
-subsection {* Proof Experiments *}
+subsection {* Validation of Soundness *}
 
-theorem SemiP_assoc :
+lemma SemiR_Semi2R_equiv_lemma1 :
+"\<lbrakk>b1 \<in> WF_BINDING;
+ b2 \<in> WF_BINDING;
+ (b1, b2) \<in> COMPOSABLE\<rbrakk> \<Longrightarrow>
+ ((b1 \<oplus> b2 on DASHED) \<oplus> (SubstB SS1 b1) on DASHED_TWICE) \<circ> SS1 =
+   b1 \<oplus> (SubstB SS1 b2) on DASHED_TWICE"
+apply (rule ext)
+apply (simp add: SubstB_def closure)
+apply (case_tac "x \<in> UNDASHED")
+apply (simp add: SS1_simps SS2_simps)
+apply (case_tac "x \<in> DASHED")
+apply (simp add: SS1_simps SS2_simps)
+apply (case_tac "x \<in> DASHED_TWICE")
+apply (simp add: SS1_simps SS2_simps)
+apply (simp add: SS1_simps SS2_simps)
+done
+
+lemma SemiR_Semi2R_equiv_lemma2 :
+"\<lbrakk>b1 \<in> WF_BINDING;
+ b2 \<in> WF_BINDING;
+ (b1, b2) \<in> COMPOSABLE\<rbrakk> \<Longrightarrow>
+ ((b1 \<oplus> b2 on DASHED) \<oplus> (SubstB SS1 b1) on DASHED_TWICE) \<circ> SS2 =
+   b2 \<oplus> (SubstB SS2 b1) on DASHED_TWICE"
+apply (rule ext)
+apply (simp add: SubstB_def closure)
+apply (case_tac "x \<in> UNDASHED")
+apply (simp add: SS1_simps SS2_simps)
+apply (simp add: COMPOSABLE_dash)
+apply (case_tac "x \<in> DASHED")
+apply (simp add: SS1_simps SS2_simps)
+apply (case_tac "x \<in> DASHED_TWICE")
+apply (simp add: SS1_simps SS2_simps)
+apply (simp add: SS1_simps SS2_simps)
+apply (simp add: COMPOSABLE_ident)
+done
+
+theorem SemiR_SemiR2_equiv :
 "\<lbrakk>p1 \<in> WF_PREDICATE;
  p2 \<in> WF_PREDICATE;
- p3 \<in> WF_PREDICATE\<rbrakk> \<Longrightarrow>
- (p1 ; p2) ; p3 = p1 ; (p2 ; p3)"
-apply (subgoal_tac "(p1 ; p2) \<in> WF_PREDICATE")
-apply (subgoal_tac "(p2 ; p3) \<in> WF_PREDICATE")
+ UNREST DASHED_TWICE p1;
+ UNREST DASHED_TWICE p2\<rbrakk> \<Longrightarrow>
+ SemiR p1 p2 = SemiR2 p1 p2"
+apply (rule sym)
+apply (simp add: SemiR2_def)
+apply (utp_pred_tac)
+apply (simp add: EvalP_def)
 apply (simp add: SemiR_def)
 apply (safe)
-(* This is still quite nasty, even in the simplified predicate model! *)
-oops
+-- {* Subgoal 1 *}
+apply (rule_tac x =
+  "SubstB (inv SS1) (b \<oplus> b' on DASHED_TWICE) \<oplus> b on DASHED_TWICE" in exI)
+apply (rule_tac x =
+  "SubstB (inv SS2) (b \<oplus> b' on DASHED_TWICE) \<oplus> b on DASHED_TWICE" in exI)
+apply (safe)
+-- {* Subgoal 1.1 *}
+apply (simp add: SubstB_def closure)
+apply (rule ext)
+apply (case_tac "x \<in> DASHED")
+apply (simp add: SS1_simps SS2_simps)
+apply (simp add: SS1_simps SS2_simps)
+apply (case_tac "x \<in> DASHED_TWICE")
+apply (simp add: SS1_simps SS2_simps)
+apply (simp add: SS1_simps SS2_simps)
+-- {* Subgoal 1.2 *}
+apply (auto intro: UNREST_member) [1]
+-- {* Subgoal 1.3 *}
+apply (auto intro: UNREST_member) [1]
+-- {* Subgoal 1.3 *}
+apply (simp add: SubstB_def closure)
+apply (simp add: COMPOSABLE_def)
+apply (safe)
+apply (simp add: SS1_simps SS2_simps)
+apply (simp add: binding_equiv_def)
+apply (simp add: NON_REL_VAR_def)
+apply (rule ballI)
+apply (clarsimp)
+apply (case_tac "x \<in> DASHED_TWICE")
+apply (simp add: SS1_simps SS2_simps)
+apply (simp add: SS1_simps SS2_simps)
+-- {* Subgoal 2 *}
+apply (simp add: SubstB_def closure)
+apply (rule_tac x = "SubstB SS1 b1" in bexI)
+apply (rule conjI)
+-- {* Subgoal 2.1 *}
+apply (simp add: SemiR_Semi2R_equiv_lemma1)
+apply (auto intro: UNREST_member simp: closure) [1]
+-- {* Subgoal 2.2 *}
+apply (simp add: SemiR_Semi2R_equiv_lemma2)
+apply (auto intro: UNREST_member simp: closure) [1]
+-- {* Subgoal 2.3 *}
+apply (simp add: closure)
+done
 end
 end
