theories/utp_meta.thy
@@ -15,6 +15,7 @@ imports utp_common
   "generic/utp_pred"
   "generic/utp_subst"
   "generic/utp_rel"
+  "generic/utp_laws"
   "utils/utp_eval_pred"
   "utils/utp_eval_rel"
 begin
